theories/utils/Library_extra/Fmap.thy
@@ -1,8 +1,6 @@
 theory Fmap
-imports HOLCF Map_Extra Fset
+imports Map_Extra Fset
 begin
-
-default_sort linorder
 
 text {* Ideally, this should only require a linear order on the domain type
         but for the sake of convenience I've got both requiring it as the
@@ -13,13 +11,28 @@ where "fmaps = Collect (finite \<circ> dom)"
 typedef (open) ('a, 'b) fmap = "fmaps :: ('a \<rightharpoonup> 'b) set" 
   by (rule_tac x="empty" in exI, simp add:fmaps_def)
 
+notation Rep_fmap ("\<langle>_\<rangle>\<^sub>m")
+
+declare Rep_fmap [simp]
+declare Rep_fmap_inverse [simp]
+declare Abs_fmap_inverse [simp]
+
+lemma Rep_fmap_intro [intro!]:
+  "Rep_fmap x = Rep_fmap y \<Longrightarrow> x = y"
+  by (simp add:Rep_fmap_inject)
+
+lemma Rep_fmap_elim [elim]:
+  "\<lbrakk> x = y; Rep_fmap x = Rep_fmap y \<Longrightarrow> P \<rbrakk> \<Longrightarrow> P"
+  by (auto)
+
 lemma Abs_fmap_inv [simp]:  "finite (dom f) \<Longrightarrow> Rep_fmap (Abs_fmap f) = f"
   apply (subgoal_tac "f \<in> fmaps")
   apply (metis Abs_fmap_inverse)
   apply (simp_all add: fmaps_def)
 done
 
-lemma Abs_fmap_inj [intro]: "\<lbrakk> Abs_fmap f = Abs_fmap g; finite (dom f); finite (dom g) \<rbrakk> \<Longrightarrow> f = g"
+lemma Abs_fmap_inj [intro]: 
+  "\<lbrakk> Abs_fmap f = Abs_fmap g; finite (dom f); finite (dom g) \<rbrakk> \<Longrightarrow> f = g"
   by (metis Abs_fmap_inv)
 
 lemma fin_dom_fmap [simp]: "finite (dom (Rep_fmap f))"
@@ -34,13 +47,37 @@ done
 
 lemma fin_map_graph_fmap [simp]: "finite (map_graph (Rep_fmap f))"
   by (metis fin_dom_fmap finite_dom_graph)
-  
-definition "fmap_list f = sorted_list_of_set (map_graph (Rep_fmap f))"
-definition "list_fmap xs = Abs_fmap (map_of xs)"
+
+setup_lifting type_definition_fmap
+
+lift_definition fdom :: "('a, 'b) fmap \<Rightarrow> 'a fset" is dom
+  by (simp add:fmaps_def fsets_def)
+
+lift_definition fran :: "('a, 'b) fmap \<Rightarrow> 'b fset" is ran
+  by (simp add:fmaps_def fsets_def)
+
+lift_definition fmempty :: "('a, 'b) fmap" is "Map.empty"
+  by (simp add:fmaps_def)
+
+lemma fdom_empty [simp]: 
+  "fdom f = \<lbrace>\<rbrace> \<Longrightarrow> f = fmempty"
+  by (auto simp add:fdom.rep_eq fmempty.rep_eq)
+
+lemma fran_empty [simp]: 
+  "fran f = \<lbrace>\<rbrace> \<Longrightarrow> f = fmempty"
+  apply (auto elim!:Rep_fset_elim simp add:fran.rep_eq fmempty.rep_eq fempty.rep_eq)
+  apply (metis empty_iff option.exhaust ranI)
+done
+
+definition "fmap_list f = map (\<lambda> x. (x, the (Rep_fmap f x))) (flist (fdom f))"
+lift_definition list_fmap :: "('a \<times> 'b) list \<Rightarrow> ('a, 'b) fmap" is "map_of"
+  by (simp add:fmaps_def finite_dom_map_of)
 
 lemma fmap_list_inv[simp]: 
   "list_fmap (fmap_list f) = f"
-  by (simp add:list_fmap_def fmap_list_def map_graph_list finite_dom_graph Rep_fmap_inverse)
+  apply (auto simp add:list_fmap.rep_eq fmap_list_def)
+  apply (metis fdom.rep_eq flist_inv fset_rep_eq map_of_map_keys)
+done
 
 lemma map_graph_set: "\<lbrakk>distinct (map fst xs); sorted xs\<rbrakk> \<Longrightarrow> set xs = map_graph (map_of xs)"
   apply (induct xs)
@@ -55,60 +92,51 @@ lemma map_graph_set: "\<lbrakk>distinct (map fst xs); sorted xs\<rbrakk> \<Longr
   apply (metis (lifting) drop_1_Cons sorted_drop)
 done
 
+lemma fdom_fmap_list [simp]: "fdom (list_fmap xs) = fset (map fst xs)"
+  by (auto simp add:fdom.rep_eq list_fmap.rep_eq dom_map_of_conv_image_fst)
+
 lemma list_fmap_inv[simp]:
-  "\<lbrakk>distinct (map fst xs); sorted xs\<rbrakk> \<Longrightarrow> fmap_list (list_fmap xs) = xs"
-  apply (simp add:list_fmap_def fmap_list_def map_graph_list finite_dom_graph Rep_fmap_inverse finite_dom_map_of)
-  apply (simp add:map_graph_set[THEN sym])
-  apply (metis (lifting) distinct_map finite_set sorted_distinct_set_unique sorted_list_of_set)
-done
+  "\<lbrakk>distinct (map fst xs); sorted (map fst xs)\<rbrakk> \<Longrightarrow> fmap_list (list_fmap xs) = xs"
+  by (auto intro!:map_idI simp add:list_fmap.rep_eq fmap_list_def map_graph_list finite_dom_graph Rep_fmap_inverse finite_dom_map_of)
+
+lemma map_fst_fmap_list [simp]:
+  "map fst (fmap_list f) = flist (fdom f)"
+  by (auto intro!:map_idI simp add:flist_def fmap_list_def)
 
 lemma fmap_list_props [simp]:
-  "sorted (fmap_list xs)"
-  "distinct (fmap_list xs)"
-  "distinct (map fst (fmap_list xs))"
-  apply (simp_all add:fmap_list_def fin_dom_fmap finite_dom_graph sorted_list_of_set)
-  apply (metis distinct_map fin_map_graph_fmap functional_def map_graph_functional sorted_list_of_set)
+  "sorted (map fst (fmap_list f))"
+  "distinct (map fst (fmap_list f))"
+  by (simp_all)
+
+lemma fmap_list_props2 [simp]:
+  "distinct (fmap_list f)"
+  by (metis (lifting) distinct_zipI1 fmap_list_props(2) zip_map_fst_snd)
+
+lemma fdom_list: "fdom f = Abs_fset (fst ` set (fmap_list f))"
+  apply (auto simp add:fdom_def fmap_list_def dom_map_graph)
+  apply (metis (lifting) fst_conv image_iff)+
 done
 
-setup_lifting type_definition_fmap
-
-lift_definition fdom :: "('a, 'b) fmap \<Rightarrow> 'a fset" is dom
-  by (simp add:fmaps_def fsets_def)
-
-lift_definition fran :: "('a, 'b) fmap \<Rightarrow> 'b fset" is ran
-  by (simp add:fmaps_def fsets_def)
-
-lemma fdom_fmap_list: "fdom f = Abs_fset (fst ` set (fmap_list f))"
-  by (simp add:fdom_def fmap_list_def dom_map_graph)
-
-lemma fran_fmap_list: "fran f = Abs_fset (snd ` set (fmap_list f))"
-  apply (simp add:fran_def fmap_list_def)
-  apply (metis fin_dom_fmap finite_dom_graph ran_map_graph sorted_list_of_set)
+lemma fran_list: "fran f = Abs_fset (snd ` set (fmap_list f))"
+  apply (auto simp add:fran.rep_eq fdom.rep_eq fmap_list_def image_def)
+  apply (auto simp add:ran_def)
 done
 
-lift_definition fmempty :: "('a, 'b) fmap" is "Map.empty"
-  by (simp add:fmaps_def)
+lemma fmext[intro]: "(\<And> x. \<langle>f\<rangle>\<^sub>m x = \<langle>g\<rangle>\<^sub>m x) \<Longrightarrow> f = g"
+  by (auto)
 
-lift_definition fmlookup :: "'a \<Rightarrow> ('a, 'b) fmap \<Rightarrow> 'b option" is "\<lambda> x f. f x"
-  by simp
+lemma fdomI: "\<langle>m\<rangle>\<^sub>m a = Some b ==> a \<in>\<^sub>f fdom m"
+  by (auto simp add:fdom_def fmember.rep_eq)
 
-lemma fmext[intro]: "(\<And> x. fmlookup x f = fmlookup x g) \<Longrightarrow> f = g"
-  apply (auto simp add:fmlookup_def)
-  apply (drule ext)
-  apply (metis Rep_fmap_inject)
-done
+lemma fdomD: "a \<in>\<^sub>f fdom m \<Longrightarrow> \<exists>b. \<langle>m\<rangle>\<^sub>m a = Some b"
+  by (auto simp add:fdom_def fmember.rep_eq)
 
-lemma fdomI: "fmlookup a m = Some b ==> a \<in>\<^sub>f fdom m"
-  by (auto simp add:fdom_def fmember.rep_eq fmlookup.rep_eq)
-
-lemma fdomD: "a \<in>\<^sub>f fdom m \<Longrightarrow> \<exists>b. fmlookup a m = Some b"
-  by (auto simp add:fdom_def fmember.rep_eq fmlookup.rep_eq)
-
-lemma fdomIff [iff, simp del]: "(a \<in>\<^sub>f fdom m) = (fmlookup a m ~= None)"
-  by (auto simp add:fdom_def fmember.rep_eq fmlookup.rep_eq)
+lemma fdomIff [iff, simp del]: "(a \<in>\<^sub>f fdom m) = (\<langle>m\<rangle>\<^sub>m a ~= None)"
+  by (auto simp add:fdom_def fmember.rep_eq)
 
 default_sort type
 
+(*
 instantiation fmap :: (type,type) discrete_cpo
 begin
 
@@ -119,5 +147,6 @@ instance proof
 qed (rule below_fmap_def)
 
 end
+*)
 
 end
