theories/models/utp_vdm_simple/utp_vdm_sorts.thy
@@ -1,0 +1,294 @@
+theory utp_vdm_sorts
+imports 
+  "../../core/utp_sorts"
+  "../../alpha/utp_alpha_pred" 
+  utp_vdm_inject 
+begin
+
+instantiation vdmval :: VALUE
+begin
+
+(*
+definition utype_rel_vval :: "vval \<Rightarrow> nat \<Rightarrow> bool" where
+"utype_rel_vval x u = \<exists> t :: vdmtype. u = emb\<cdot>(Def t) \<and> x :\<^sub>v t)"
+*)
+
+definition utype_rel_vdmval :: "vdmval \<Rightarrow> nat \<Rightarrow> bool" where
+"utype_rel_vdmval x u = (\<exists> t :: vdmtype. u = to_nat t \<and> x :\<^sub>v t)"
+
+definition Defined_vdmval :: "vdmval \<Rightarrow> bool" where
+"Defined_vdmval x \<equiv> x \<noteq> BotV"
+
+instance
+  apply (intro_classes)
+  apply (simp add:utype_rel_vdmval_def Defined_vdmval_def)
+  apply (rule_tac x="to_nat BoolT" in exI)
+  apply (force)
+done
+end
+
+lemma Defined_BasicV [simp]: "\<D> (BasicV x)"
+  by (simp add:Defined_vdmval_def)
+
+lemma vdmtype_UTYPE [simp]: "\<lbrakk> v :\<^sub>v t; \<D> v \<rbrakk> \<Longrightarrow> to_nat t \<in> UTYPES (TYPE(vdmval))"
+  by (auto simp add:UTYPES_def utype_rel_vdmval_def)
+
+lemma prjTYPE_inv_vdm [simp]
+  : "embTYPE ((prjTYPE t) :: vdmtype) = (t :: vdmval UTYPE)"
+  apply (simp add:prjTYPE_def embTYPE_def)
+  apply (case_tac t)
+  apply (auto simp add: utype_rel_vdmval_def UTYPES_def)
+done
+
+lemma type_rel_vdmtype_exists: 
+  "(x::vdmval) : a \<Longrightarrow> \<exists> t. a = embTYPE t \<and> x :\<^sub>v t" 
+  apply (simp add:type_rel_def)
+  apply (simp add:utype_rel_vdmval_def)
+  apply (case_tac a)
+  apply (auto simp add:UTYPES_def)
+  apply (rule_tac x="t" in exI)
+  apply (simp add:embTYPE_def)
+done
+
+lemma type_rel_vdmtype_elim [elim]:
+  "\<lbrakk>(x::vdmval) : a; \<And> t. a = embTYPE t \<and> x :\<^sub>v t \<Longrightarrow> P \<rbrakk> \<Longrightarrow> P"
+  by (metis type_rel_vdmtype_exists)
+
+lemma type_rel_vdmtype [simp]: "x : t \<longleftrightarrow> x :\<^sub>v prjTYPE t"
+  apply (auto)
+  apply (erule type_rel_vdmtype_elim)
+  apply (auto)
+  apply (metis BotV_type Defined_vdmval_def embTYPE_inv utype_rel_vdmval_def)
+  apply (simp add:type_rel_def utype_rel_vdmval_def)
+  apply (rule_tac x="prjTYPE t" in exI)
+  apply (simp add:prjTYPE_def)
+  apply (case_tac t)
+  apply (auto simp add:UTYPES_def utype_rel_vdmval_def)
+done
+
+instantiation vdmval :: BOT_SORT
+begin
+
+definition ubot_vdmval :: "vdmval" where
+"ubot_vdmval = BotV"
+
+instance
+  apply (intro_classes)
+  apply (simp add:ubot_vdmval_def Defined_vdmval_def)
+done
+end
+
+lemma Defined_bot [simp]: "\<D> (BotV :: vdmval) \<longleftrightarrow> False"
+  by (simp add:Defined_vdmval_def)
+
+lemma Defined_ubot [simp]: "\<D> \<bottom>v \<longleftrightarrow> False"
+  by (simp add:Defined_vdmval_def)
+
+(*
+lemma vdmval_UTYPE_nbot [simp]: 
+  "(from_nat (Rep_UTYPE (t :: vdmval UTYPE)) :: vdmtype lift) \<noteq> \<bottom>"
+  apply (case_tac t)
+  apply (auto simp add: UTYPES_def utype_rel_vdmval_def)
+  apply (auto)
+done
+
+lemma vdmval_UTYPE_Def [simp]: 
+  "\<exists> x. (prj\<cdot>(Rep_UTYPE (a :: vdmval UTYPE)) :: vdmtype lift) = Def x"
+  apply (case_tac a)
+  apply (simp add: UTYPES_def)
+  apply (simp add: utype_rel_vdmval_def)
+  apply (auto)
+done
+
+lemma vdmval_UTYPE_elim [elim]:
+  assumes "\<And> x. (prj\<cdot>(Rep_UTYPE (a :: vdmval UTYPE)) :: vdmtype lift) = Def x \<Longrightarrow> P" 
+  shows "P"
+  by (metis assms vdmval_UTYPE_Def)
+*)
+subsection {* Int sort instantiation *}
+
+instantiation vdmval :: INT_SORT
+begin
+
+definition MkInt_vdmval where "MkInt_vdmval (x::int) = InjVB x"
+definition DestInt_vdmval where "DestInt_vdmval x = (ProjVB x :: int)"
+definition IntUType_vdmval :: "vdmval itself \<Rightarrow> nat" where 
+"IntUType_vdmval = (\<lambda> x. to_nat IntT)"
+
+instance 
+  apply (intro_classes, simp_all add:MkInt_vdmval_def DestInt_vdmval_def IntUType_vdmval_def type_rel_def utype_rel_vdmval_def embTYPE_def)
+  apply (auto)
+  apply (simp_all add: Inject_int_def InjVB_def Defined_vdmval_def MkInt_vdmval_def image_def)
+  apply (force)+
+done
+end
+
+subsection {* Bool sort instantiation *}
+
+instantiation vdmval :: BOOL_SORT
+begin
+
+definition MkBool_vdmval where "MkBool_vdmval (x::bool) = InjVB x"
+definition DestBool_vdmval where "DestBool_vdmval x = (ProjVB x :: bool)"
+definition BoolUType_vdmval :: "vdmval itself \<Rightarrow> nat" where 
+"BoolUType_vdmval = (\<lambda>x. to_nat BoolT)"
+
+instance 
+  apply (intro_classes, simp_all add:MkBool_vdmval_def DestBool_vdmval_def BoolUType_vdmval_def type_rel_def utype_rel_vdmval_def embTYPE_def)
+  apply (auto)
+  apply (simp_all add:InjVB_def Inject_bool_def Defined_vdmval_def MkBool_vdmval_def image_def)
+  apply (force)
+  apply (erule vbtypes_type_cases)
+  apply (auto)
+done
+end
+
+subsection {* Set sort instantiation *}
+
+instantiation vdmval :: SET_SORT_PRE
+begin
+
+  definition MkSet_vdmval :: "vdmval set \<Rightarrow> vdmval" where
+  "MkSet_vdmval xs = SetV (ProjBasicV ` xs)"
+  
+  definition DestSet_vdmval :: "vdmval \<Rightarrow> vdmval set" where
+  "DestSet_vdmval v = BasicV ` ProjSetV v"
+
+  definition IsSetElemType_vdmval :: "vdmval UTYPE \<Rightarrow> bool" where
+  "IsSetElemType_vdmval t = (prjTYPE t \<in> vbtypes)"
+
+  definition SetType_vdmval :: "vdmval UTYPE \<Rightarrow> vdmval UTYPE" where
+  "SetType_vdmval t = embTYPE (SetT (prjTYPE t))"
+
+instance ..
+
+end
+
+instantiation vdmval :: SET_SORT
+begin
+
+instance
+  apply (intro_classes)
+  apply (auto simp add:DestSet_vdmval_def MkSet_vdmval_def SetType_vdmval_def IsSetElemType_vdmval_def)
+  apply (drule_tac x="xb" in bspec)
+  apply (simp)
+  apply (force)
+  apply (force)
+  apply (simp_all add:dcarrier_def)
+  apply (auto)
+  apply (subgoal_tac "\<exists> v::vdmval. v :\<^sub>u to_nat (SetT (prjTYPE t)) \<and> \<D> v")
+  apply (force)
+  apply (rule_tac x="SetV {}" in exI)
+  apply (auto simp add:utype_rel_vdmval_def Defined_vdmval_def)
+  apply (subgoal_tac "\<exists> v::vdmval. v :\<^sub>u to_nat (SetT (prjTYPE t)) \<and> \<D> v")
+  apply (auto simp add:image_def MkSet_vdmval_def utype_rel_vdmval_def Defined_vdmval_def)
+  apply (erule SetT_type_cases)
+  apply (simp)
+  apply (auto)
+  apply (rule_tac x="BasicV ` xs" in bexI)
+  apply (auto)
+done
+
+end
+
+(*
+instantiation vdmval :: FUNCTION_SORT
+begin
+
+definition MkFunc_vdmval where "MkFunc_vdmval f = FuncV\<cdot>(\<Lambda>! x. f x)"
+definition DestFunc_vdmval where "DestFunc_vdmval f \<equiv> \<lambda> x. (sfun_rep\<cdot>(ProjFuncV\<cdot>f))\<cdot>x"
+definition IsFunc_vdmval :: "(vdmval \<Rightarrow> vdmval) \<Rightarrow> bool" where
+"IsFunc_vdmval f \<equiv> cont f \<and> f \<bottom> = \<bottom> \<and> (\<exists>x. x \<noteq> \<bottom> \<and> f x \<noteq> \<bottom>)"
+definition FuncType_vdmval :: "vdmval UTYPE \<Rightarrow> vdmval UTYPE \<Rightarrow> vdmval UTYPE" where
+"FuncType_vdmval a b \<equiv>
+  case (prj\<cdot>(Rep_UTYPE a), prj\<cdot>(Rep_UTYPE b)) of
+    (Def a', Def b') \<Rightarrow> embTYPE (FuncT a' b') |
+    _ \<Rightarrow> Abs_UTYPE (emb\<cdot>(\<bottom> :: vdmtype lift))"
+
+instance proof
+  fix f :: "vdmval \<Rightarrow> vdmval"
+
+  assume isFunc: "IsFunc f"
+  from isFunc show "DestFunc (MkFunc f) = f"
+    by (simp add:MkFunc_vdmval_def DestFunc_vdmval_def IsFunc_vdmval_def)
+
+  from isFunc show "\<D> (MkFunc f)"
+    apply (auto simp add:Defined_vdmval_def IsFunc_vdmval_def MkFunc_vdmval_def FuncType_vdmval_def sfun_eq_iff)
+    apply (metis Abs_cfun_inverse2 Rep_cfun_strict1)
+  done
+
+  fix a b :: "vdmval UTYPE"
+  assume funcRange: "\<forall>x. x : a \<longrightarrow> f x : b"
+  from isFunc funcRange show "MkFunc f : FuncType a b"
+    apply (auto simp add: MkFunc_vdmval_def type_rel_def utype_rel_vdmval_def IsFunc_vdmval_def)
+    apply (simp add:FuncType_vdmval_def)
+    apply (insert vdmval_UTYPE_Def[of "a"])
+    apply (erule exE)
+    apply (simp)
+    apply (insert vdmval_UTYPE_Def[of "b"])
+    apply (erule exE)
+    apply (simp add:embTYPE_def)
+
+    apply (rule FuncV_type)
+    apply (auto)
+    apply (metis (lifting) BasicV_type Rep_UTYPE_elim emb_inverse lift.inject utype_rel_vdmval_def)
+  done
+qed
+end
+
+
+
+lemma carrier_vcarrier [simp]: "carrier t = vcarrier (prjTYPE t)"
+  by (simp add:carrier_def vcarrier_def)
+
+lemma prjTYPE_vdmval_IntT [simp]: 
+  "prjTYPE (IntType :: vdmval UTYPE) = IntT"
+  by (auto intro!: embTYPE_inv simp add:utype_rel_vdmval_def IntType_vdmval_def)
+
+lemma prjTYPE_vdmval_BoolT [simp]: 
+  "prjTYPE (BoolType :: vdmval UTYPE) = BoolT"
+  by (auto intro!: embTYPE_inv simp add:utype_rel_vdmval_def BoolType_vdmval_def)
+
+lemma prjTYPE_vdmval_FuncT [simp]:
+  "prjTYPE (FuncType a b :: vdmval UTYPE) = prjTYPE a → prjTYPE b"
+  apply (case_tac a)
+  apply (simp)
+  apply (simp add:FuncType_vdmval_def)
+  apply (insert vdmval_UTYPE_Def[of a])
+  apply (insert vdmval_UTYPE_Def[of b])
+  apply (erule exE)
+  apply (erule exE)
+  apply (simp)
+  apply (auto)
+  apply (metis Abs_UTYPE_inverse Undef.simps embTYPE_def emb_inverse prjTYPE_def vdmtype_UTYPE)
+done
+*)
+
+definition binding_fmap ::
+  "'VALUE WF_BINDING \<Rightarrow> 'VALUE ALPHABET \<Rightarrow> ('VALUE VAR, 'VALUE) fmap" where
+"binding_fmap b a = list_fmap (map (\<lambda> x. (x, \<langle>b\<rangle>\<^sub>b x)) (flist a))"
+
+lemma "Fmap.fdom (binding_fmap b a) = a"
+  apply (simp add:binding_fmap_def)
+  oops
+
+definition fmap_binding ::
+  "('VALUE VAR, 'VALUE) fmap \<Rightarrow> 'VALUE WF_BINDING" where
+"fmap_binding f = Abs_WF_BINDING (\<lambda> x. if (x \<in>\<^sub>f Fmap.fdom f) then the (\<langle>f\<rangle>\<^sub>m x) else default (vtype x))"
+
+lemma "fmap_binding (binding_fmap b a) \<cong> b on \<langle>a\<rangle>\<^sub>f"
+  oops
+
+
+(*
+definition predicate_lists :: 
+  "'VALUE WF_PREDICATE \<Rightarrow> 'VALUE ALPHABET \<Rightarrow> ('VALUE list) set" where
+"predicate_lists p a = (\<lambda> b. map \<langle>b\<rangle>\<^sub>b (flist a)) ` destPRED p"
+
+definition lists_predicate :: 
+  "('VALUE list) set \<Rightarrow> 'VALUE ALPHABET \<Rightarrow> 'VALUE WF_PREDICATE" where
+"lists_predicate vs a = mkPRED {b. }"
+*)
+
+
+end
