theories/models/utp_vdm_simple/utp_vdm_values.thy
@@ -1,0 +1,333 @@
+(******************************************************************************)
+(* Project: VDM model for Isabelle/UTP                                        *)
+(* File: utp_vdm_values.thy                                                   *)
+(* Author: Simon Foster, University of York (UK)                              *)
+(******************************************************************************)
+theory utp_vdm_values
+imports 
+   Derive
+  "~~/src/HOL/Library/Char_ord" 
+  "~~/src/HOL/Library/Monad_Syntax" 
+  "../../core/utp_var"
+  "../../utils/Library_extra"
+
+begin
+
+section {* Main domain types *}
+
+subsection {* Basic (countable) values *}
+
+text {* We introduce countable values using a normal datatype. This representation
+  is not fully canonical, as we use lists to represents sets, maps and records.
+  However, we later introduce constructors for these which use the correct types
+  and thus ensure canonicity. *}
+datatype vbasic 
+  = PairI vbasic vbasic
+  | NatI "nat"
+  | IntI "int" 
+  | RatI "rat" 
+  | CharI "char"
+  | QuoteI "string" 
+  | TokenI vbasic
+  | ListI "vbasic list" 
+  | FinI "vbasic list"
+  | BoolI bool
+  | RecI "vbasic list"
+  | MapI "(vbasic * vbasic) list" 
+
+(* Deriving the linear order necessarily takes a while *)
+
+(*
+derive linorder vbasic
+*)
+
+instantiation vbasic :: linorder
+begin
+
+instance sorry
+
+end
+
+derive countable vbasic
+
+subsection {* Full values *}
+
+text {* Full values are represented using a domain, which adds functions, 
+  uncountable sets, reals etc. to what we already have. Domains are harder to
+  manipulate than datatypes so we only use them where necessary. Functions
+  and sets must have a continuous representation, but since vbasic is "flat"
+  any function whose domain is vbasic is automatically continuous.
+*}
+
+datatype vdmval = SetV "vbasic set"
+                | FuncV "vbasic \<Rightarrow> vdmval"
+                | BasicV "vbasic"
+                | BotV
+
+abbreviation "TrueV \<equiv> BasicV (BoolI True)"
+abbreviation "FalseV \<equiv> BasicV (BoolI False)"
+
+subsection {* Injections *}
+
+text {* We create interface constructors for finite sets, maps and records which
+  use derived subtypes as inputs and therefore preserve canonicity of vbasic *}
+
+definition FSetI :: "vbasic fset \<Rightarrow> vbasic" where
+"FSetI vs = FinI (flist vs)"
+
+definition FinMapI :: "(vbasic, vbasic) fmap \<Rightarrow> vbasic" where
+"FinMapI f = MapI (fmap_list f)"
+
+(*
+definition RecordI :: "(string \<rightharpoonup> vbasic) \<Rightarrow> vbasic" where
+"RecordI f = RecI (sorted_list_of_set (map_graph f))"
+*)
+
+subsection {* Projections *}
+
+text {* Projections functions produce Some value for a correctly formed values,
+  and None otherwise *}
+
+fun ProjFSetI :: "vbasic \<Rightarrow> (vbasic fset) option" where
+"ProjFSetI (FinI xs) = Some (fset xs)" |
+"ProjFSetI x = None"
+
+fun ProjPairI :: "vbasic \<Rightarrow> (vbasic * vbasic) option" where
+"ProjPairI (PairI x y) = Some (x,y)" | "ProjPairI x = None"
+
+fun ProjRatI :: "vbasic \<Rightarrow> rat option" where
+"ProjRatI (RatI x) = Some x" | "ProjRatI x = None"
+
+fun ProjIntI :: "vbasic \<Rightarrow> int option" where
+"ProjIntI (IntI x) = Some x" | "ProjIntI x = None"
+
+fun ProjCharI :: "vbasic \<Rightarrow> char option" where
+"ProjCharI (CharI x) = Some x" | "ProjCharI x = None"
+
+fun ProjBoolI :: "vbasic \<Rightarrow> bool option" where
+"ProjBoolI (BoolI x) = Some x" | "ProjBoolI x = None"
+
+fun ProjListI :: "vbasic \<Rightarrow> (vbasic list) option" where
+"ProjListI (ListI xs) = Some xs" | "ProjListI xs = None"
+
+fun ProjMapI :: "vbasic \<Rightarrow> ((vbasic* vbasic) list) option" where
+"ProjMapI (MapI f) = Some f" | "ProjMapI x = None"
+
+fun ProjFinMapI :: "vbasic \<Rightarrow> ((vbasic, vbasic) fmap) option" where
+"ProjFinMapI (MapI xs) = Some (list_fmap xs)" | "ProjFinMapI x = None"
+
+lemma FinMapI_inj [simp]: "FinMapI f = FinMapI g \<Longrightarrow> f = g"
+  apply (auto simp add: FinMapI_def)
+  apply (metis fmap_list_inv)
+done
+
+section {* The type-system *}
+
+subsection {* Types *}
+
+text {* We only introduce a single datatype for types, as the move between vdmval and
+  vbasic should be transparent *}
+
+datatype vdmtype =
+    FSetT vdmtype
+  | MapT vdmtype vdmtype 
+  | ListT vdmtype
+  | PairT vdmtype vdmtype 
+  | RecordT "vdmtype list"
+  | BoolT ("\<bool>")
+  | NatT ("\<nat>")
+  | IntT ("\<int>")
+  | RatT ("\<rat>")
+  | CharT
+  | QuoteT "string fset"
+  | TokenT
+  | VarT nat
+  | SetT vdmtype 
+  | FuncT vdmtype vdmtype (infixr "→" 60)
+
+derive countable vdmtype
+
+subsection {* Basic value typing relation *}
+
+inductive vbasic_type_rel :: "vbasic \<Rightarrow> vdmtype \<Rightarrow> bool" (infix ":\<^sub>b" 50) 
+  and vbasic_type_list_rel :: "vbasic list \<Rightarrow> vdmtype list \<Rightarrow> bool" (infix ":\<^sub>r" 50) where
+BoolI_type[intro]: "BoolI x :\<^sub>b BoolT" |
+NatI_type[intro]: "NatI x :\<^sub>b NatT" |
+IntI_type[intro]: "IntI x :\<^sub>b IntT" |
+RatI_type[intro]: "RatI x :\<^sub>b RatT" |
+CharI_type[intro]: "CharI x :\<^sub>b CharT" |
+TokenI_type[intro]: "TokenI x :\<^sub>b TokenT" |
+QuoteI_type[intro]: "x \<in>\<^sub>f xs \<Longrightarrow> QuoteI x :\<^sub>b QuoteT xs" |
+ListI_type[intro]: "\<lbrakk> \<forall>x\<in>set xs. x :\<^sub>b a \<rbrakk> \<Longrightarrow> ListI xs :\<^sub>b ListT a" |
+FinI_type[intro]: "\<lbrakk> \<forall>x\<in>set xs. x :\<^sub>b a; sorted xs; distinct xs \<rbrakk> \<Longrightarrow> FinI xs :\<^sub>b FSetT a" |
+PairI_type[intro]: "\<lbrakk> x :\<^sub>b a; y :\<^sub>b b \<rbrakk> \<Longrightarrow> PairI x y :\<^sub>b PairT a b" |
+MapI_type[intro]: "\<lbrakk> \<forall>(x,y)\<in>set xs. x :\<^sub>b a \<and> y :\<^sub>b b; sorted (map fst xs); distinct (map fst xs) \<rbrakk> \<Longrightarrow> MapI xs :\<^sub>b MapT a b" |
+RecI_type[intro]: "\<lbrakk> xs :\<^sub>r ts \<rbrakk>  \<Longrightarrow> RecI xs :\<^sub>b RecordT ts" |
+Cons_type[intro]: "\<lbrakk> x :\<^sub>b t; xs :\<^sub>r ts \<rbrakk> \<Longrightarrow> (x # xs) :\<^sub>r (t # ts)" |
+Nil_type[intro]: "[] :\<^sub>r []"
+
+inductive_cases 
+  BoolI_type_cases [elim]: "BoolI x :\<^sub>b t" and
+  BoolT_type_cases [elim!]: "x :\<^sub>b BoolT" and
+  NatI_type_cases [elim]: "NatI x :\<^sub>b t" and
+  NatT_type_cases [elim!]: "x :\<^sub>b NatT" and
+  IntI_type_cases [elim]: "IntI x :\<^sub>b t" and
+  IntT_type_cases [elim!]: "x :\<^sub>b IntT" and
+  RatI_type_cases [elim]: "RatI x :\<^sub>b t" and
+  RatT_type_cases [elim!]: "x :\<^sub>b RatT" and
+  CharI_type_cases [elim]: "CharI x :\<^sub>b t" and
+  CharT_type_cases [elim!]: "x :\<^sub>b CharT" and
+  TokenI_type_cases [elim]: "TokenI x :\<^sub>b t" and
+  TokenT_type_cases [elim!]: "x :\<^sub>b TokenT" and
+  QuoteI_type_cases [elim]: "QuoteI x :\<^sub>b t" and
+  QuoteT_type_cases [elim!]: "x :\<^sub>b QuoteT xs" and
+  ListI_type_cases [elim]: "ListI xs :\<^sub>b t" and
+  ListT_type_cases [elim!]: "x :\<^sub>b ListT a" and
+  FinI_type_cases [elim]: "FinI x :\<^sub>b t" and
+  FinT_type_cases [elim!]: "x :\<^sub>b FSetT a" and
+  PairI_type_cases [elim]: "PairI x y :\<^sub>b t" and
+  PairT_type_cases [elim!]: "x :\<^sub>b PairT a b" and
+  MapI_type_cases [elim]: "MapI xs :\<^sub>b t" and
+  MapT_type_cases [elim!]: "x :\<^sub>b MapT a b" and
+  RecI_type_cases [elim]: "RecI xs :\<^sub>b t" and
+  RecT_type_cases [elim!]: "x :\<^sub>b RecordT fs" and
+  Cons_type_cases [elim!]: "x :\<^sub>r f # fs" and
+  Nil_type_cases [elim!]: "x :\<^sub>r []" and
+  FuncT_type_casesB [elim!]: "x :\<^sub>b a → b" and
+  SetT_type_casesB [elim!]: "x :\<^sub>b SetT a"
+
+definition bcarrier :: "vdmtype \<Rightarrow> vbasic set" where
+"bcarrier t = {x. x :\<^sub>b t}"
+
+definition vbtypes :: "vdmtype set" where
+"vbtypes = {t. \<exists> x. x :\<^sub>b t}"
+
+definition vbvalues :: "vdmval set" where
+"vbvalues = {BasicV x | x t. x :\<^sub>b t}"
+
+lemma vbtypes_simps [simp]:
+  "\<nat> \<in> vbtypes" "\<int> \<in> vbtypes" "\<rat> \<in> vbtypes"
+  "\<bool> \<in> vbtypes" "CharT \<in> vbtypes" "TokenT \<in> vbtypes"
+  "a → b \<notin> vbtypes"
+  "SetT a \<notin> vbtypes"
+  by (auto simp add:vbtypes_def)
+
+text {* We introduce a couple of derived typing rules *}
+
+lemma NilI_type[intro]: "ListI [] :\<^sub>b ListT a"
+  by auto
+
+lemma ConsI_type[intro]: 
+  "\<lbrakk> x :\<^sub>b a; ListI xs :\<^sub>b ListT a \<rbrakk> \<Longrightarrow> ListI (x # xs) :\<^sub>b ListT a"
+  by (force intro!: ListI_type)
+
+lemma FSetI_type[intro]:
+  assumes sty: "\<forall>x\<in>set (flist xs). x :\<^sub>b a" 
+  shows "FSetI xs :\<^sub>b FSetT a"
+  by (auto simp add:FSetI_def sty)
+
+lemma FinMapI_type[intro]: 
+  "\<lbrakk> \<forall> x\<in>Rep_fset(fdom f). x :\<^sub>b a; \<forall> y\<in>Rep_fset(fran f). y :\<^sub>b b \<rbrakk> \<Longrightarrow> FinMapI f :\<^sub>b MapT a b"
+  by (auto intro!:MapI_type simp add:fdom_list fran_list FinMapI_def)
+
+lemma dom_map_of: "x \<in> dom (map_of xs) \<Longrightarrow> \<exists> y. (x,y) \<in> set xs"
+  by (auto dest:map_of_SomeD simp add:dom_def)
+
+lemma ran_map_of: "y \<in> ran (map_of xs) \<Longrightarrow> \<exists> x. (x,y) \<in> set xs"
+  by (auto dest:map_of_SomeD simp add:ran_def)
+
+lemma FinMapI_type_cases [elim!]:
+  "\<lbrakk>x :\<^sub>b MapT a b; \<And>f. \<lbrakk>x = FinMapI f; \<forall> x\<in>Rep_fset(fdom f). x :\<^sub>b a; \<forall> y\<in>Rep_fset(fran f). y :\<^sub>b b \<rbrakk> \<Longrightarrow> P\<rbrakk> \<Longrightarrow> P"
+  apply (case_tac x, auto elim!:MapI_type_cases)
+  apply (simp add:FinMapI_def fdom_def fran_def)
+  apply (subgoal_tac "list = fmap_list (list_fmap list)")
+  apply (subgoal_tac "\<forall>x\<in>dom (Rep_fmap (list_fmap list)). x :\<^sub>b a")
+  apply (subgoal_tac "\<forall>y\<in>ran (Rep_fmap (list_fmap list)). y :\<^sub>b b")
+  apply (metis)
+  apply (simp add: list_fmap_def finite_dom_map_of)
+  apply (force dest: ran_map_of)
+  apply (simp add: list_fmap_def finite_dom_map_of)
+  apply (rule ballI)
+  apply (drule dom_map_of)
+  apply (force)
+  apply (simp)
+done
+  
+subsection {* Full value typing relation *}
+
+(* At the moment the type-system only supports functions of type vbtype \<Rightarrow> vdmtype.
+   Treatment of higher-order functions needs more work *)
+
+inductive vdmtype_rel :: "vdmval \<Rightarrow> vdmtype \<Rightarrow> bool" (infix ":\<^sub>v" 50) where
+BotV_type[intro]: "BotV :\<^sub>v a" |
+SetV_type[intro]: "\<lbrakk> \<forall> x\<in>xs. x :\<^sub>b a \<rbrakk> \<Longrightarrow> SetV xs :\<^sub>v SetT a" |
+BasicV_type[intro]: "x :\<^sub>b a \<Longrightarrow> BasicV x :\<^sub>v a" |
+FuncV_type[intro]: "\<lbrakk> \<forall> x. x :\<^sub>b a \<longrightarrow> f x :\<^sub>v b \<rbrakk> \<Longrightarrow> FuncV f :\<^sub>v a → b"
+
+inductive_cases
+  BotV_type_cases[elim]: "BotV :\<^sub>v a" and
+  SetT_type_cases[elim]: "x :\<^sub>v SetT a" and
+  SetV_type_cases[elim!]: "SetV x :\<^sub>v t" and
+  FuncT_type_cases[elim!]: "x :\<^sub>v a → b" and
+  FuncI_type_cases[elim!]: "FuncV f :\<^sub>v t" and
+  BasicV_type_cases[elim]: "BasicV x :\<^sub>v t"
+
+lemma vbtypes_type_cases [elim]: 
+  "\<lbrakk> a :\<^sub>v t; t \<in> vbtypes; \<And> x. \<lbrakk> a = BasicV x; x :\<^sub>b t \<rbrakk> \<Longrightarrow> P; a = BotV \<Longrightarrow> P \<rbrakk> \<Longrightarrow> P"
+  apply (case_tac a)
+  apply (auto elim:BasicV_type_cases simp add:vbtypes_def)
+done
+
+definition vcarrier :: "vdmtype \<Rightarrow> vdmval set" where
+"vcarrier t = {x. x :\<^sub>v t}"
+
+lemma vcarrier [simp]: "x :\<^sub>v t \<Longrightarrow> x \<in> vcarrier t"
+  by (simp add:vcarrier_def)
+
+lemma vcarrier_simps [simp]:
+  "vcarrier \<nat> = {BotV} \<union> {BasicV (NatI x) | x . True}"
+  "vcarrier \<int> = {BotV} \<union> {BasicV (IntI x) | x . True}"
+  "vcarrier \<rat> = {BotV} \<union> {BasicV (RatI x) | x . True}"
+  "vcarrier \<bool> = {BotV} \<union> {BasicV (BoolI x) | x . True}"
+  by (auto simp add:vcarrier_def)
+
+lemma vbvalues_vbtypes [simp]: 
+  "\<lbrakk> x \<in> vbvalues; x :\<^sub>v t \<rbrakk> \<Longrightarrow> t \<in> vbtypes"
+  by (auto simp add:vbvalues_def vbtypes_def)
+
+(* Flatness of vbasic values *)
+
+subsection {* Injecting basic values into vdmval *}
+
+primrec ProjBasicV :: "vdmval \<Rightarrow> vbasic" where
+"ProjBasicV (BasicV x) = x"
+
+fun IsBasicV :: "vdmval \<Rightarrow> bool" where
+"IsBasicV (BasicV x) = True" |
+"IsBasicV _ = False"
+
+lemma ProjBasicV_inv [simp] :
+  "IsBasicV x \<Longrightarrow> BasicV (ProjBasicV x) = x"
+  by (case_tac x, simp_all)
+
+definition vbasic_fun1 :: "(vbasic \<Rightarrow> vbasic) \<Rightarrow> vdmval" where
+"vbasic_fun1 f \<equiv> FuncV (BasicV \<circ> f)"
+
+definition vbasic_fun2 :: "(vbasic \<Rightarrow> vbasic \<Rightarrow> vbasic) \<Rightarrow> vdmval" where
+"vbasic_fun2 f \<equiv> FuncV (\<lambda> x. FuncV (\<lambda> y. BasicV (f x y)))"
+
+primrec ProjFuncV :: "vdmval \<Rightarrow> (vbasic \<Rightarrow> vdmval)" where
+"ProjFuncV (FuncV f) = f"
+
+fun IsFuncV :: "vdmval \<Rightarrow> bool" where
+"IsFuncV (FuncV f) = True" |
+"IsFuncV _ = False"
+
+primrec ProjSetV :: "vdmval \<Rightarrow> vbasic set" where
+"ProjSetV (SetV x) = x"
+
+fun IsSetV :: "vdmval \<Rightarrow> bool" where
+"IsSetV (SetV x) = True" |
+"IsSetV _ = False"
+
+end
